fstar/MLS.Test.FromExt.TreeKEM.fst
@@ -103,7 +103,7 @@ let gen_treekem_output #cb t =
     let root_secret_after_update = extract_result (root_secret tk2 my_index my_leaf_secret) in
 
     let ratchet_tree2 = extract_result (treesync_to_ratchet_tree ts2) in
-    let byte_length_ratchet_tree2 = bytes_length (ps_option (ps_node_nt _)) (Seq.seq_to_list ratchet_tree2) in
+    let byte_length_ratchet_tree2 = bytes_length (ps_option (ps_node_nt _)) ratchet_tree2 in
     let ratchet_tree_after = if 1 <= byte_length_ratchet_tree2 && byte_length_ratchet_tree2 < pow2 30 then (ps_to_pse (ps_ratchet_tree_nt _)).serialize_exact ratchet_tree2 else empty in
     let tree_hash_after = extract_result (tree_hash ts2) in
     {
