fstar/MLS.TreeKEM.NetworkTypes.fst
@@ -21,14 +21,14 @@ noeq type hpke_ciphertext_nt (bytes:Type0) {|bytes_like bytes|} = {
 
 noeq type update_path_node_nt (bytes:Type0) {|bytes_like bytes|} = {
   encryption_key: hpke_public_key_nt bytes;
-  encrypted_path_secret: mls_seq bytes ps_hpke_ciphertext_nt;
+  encrypted_path_secret: mls_list bytes ps_hpke_ciphertext_nt;
 }
 
 %splice [ps_update_path_node_nt] (gen_parser (`update_path_node_nt))
 
 noeq type update_path_nt (bytes:Type0) {|bytes_like bytes|} = {
   leaf_node: leaf_node_nt bytes tkt;
-  nodes: mls_seq bytes ps_update_path_node_nt;
+  nodes: mls_list bytes ps_update_path_node_nt;
 }
 
 %splice [ps_update_path_nt] (gen_parser (`update_path_nt))
